@prefix : <http://www.perspectum.com/ontology/scanner#> .
@prefix owl: <http://www.w3.org/2002/07/owl#> .
@prefix rdf: <http://www.w3.org/1999/02/22-rdf-syntax-ns#> .
@prefix xml: <http://www.w3.org/XML/1998/namespace> .
@prefix xsd: <http://www.w3.org/2001/XMLSchema#> .
@prefix muom: <http://www.perspectum.com/ontology/metricUoM#> .
@prefix qudt: <http://qudt.org/schema/qudt#> .
@prefix rdfs: <http://www.w3.org/2000/01/rdf-schema#> .
@prefix unit: <http://qudt.org/vocab/unit#> .
@base <http://www.perspectum.com/ontology/metricUoM> .

<http://www.perspectum.com/ontology/metricUoM> rdf:type owl:Ontology ;
                                                owl:versionIRI <http://www.perspectum.com/ontology/metricUoM/1.0> ;
                                                rdfs:comment """An Ontology to model metric Unit of Measure information.  This ontology models the house Units of Measure preferred for each metric collected in Perspectum biomedical studies. To be used initially in support of an ontology of metrics collected in a clinical study of multi-organ imaging of  patients exhibiting symptoms of long Covid.

Perspectum has published a  longitudinal, observational clinical study (Dennis et al, 2020) of patients, still experiencing  symptoms 3 months post-infection, with acute SARS-CoV-2. Patients were assessed with health  questionnaires, blood investigations and quantitative magnetic resonance imaging (MRI). 

Dennis, A. et al. (2020) ‘Multi-organ impairment in low-risk individuals with long COVID’, medRxiv, p. 2020.10.14.20212555. doi: 10.1101/2020.10.14.20212555.""" ;
                                                rdfs:seeAlso """http://www.perspectum.com/ontology/metrics
http://www.perspectum.com/ontology/scanner""" ;
                                                owl:versionInfo """Versions

3/8/2021 1.0  First version""" .

#################################################################
#    Object Properties
#################################################################

###  http://www.perspectum.com/ontology/metricUoM#hasDefaultUnit
muom:hasDefaultUnit rdf:type owl:ObjectProperty ;
                    owl:inverseOf muom:isDefaultUnitForType ;
                    rdfs:comment "Within Perspectum, this relationship defines the types of metric collected in studies with a specific unit of measure as its default ." ;
                    rdfs:label "has default unit of measure" .


###  http://www.perspectum.com/ontology/metricUoM#isDefaultUnitForType
muom:isDefaultUnitForType rdf:type owl:ObjectProperty ;
                          rdfs:domain muom:DefaultUoM ;
                          rdfs:range muom:MetricType ;
                          rdfs:comment "Within Perspectum, this relationship defines the default unit of measure for a specific type of metric collected in studies." ;
                          rdfs:label "is default unit for metric type" .


#################################################################
#    Classes
#################################################################

###  http://qudt.org/schema/qudt#Unit
qudt:Unit rdf:type owl:Class ;
          rdfs:comment "A unit from the QUDT units of measure ontology." ;
          rdfs:label "QUDT unit" .


###  http://www.perspectum.com/ontology/metricUoM#DefaultUoM
muom:DefaultUoM rdf:type owl:Class ;
                rdfs:subClassOf qudt:Unit ;
                owl:disjointWith muom:MetricType ;
                rdfs:comment "The default unit of measure for this type of metric in Perspectum study data." ;
                rdfs:label "default UoM" .


###  http://www.perspectum.com/ontology/metricUoM#MetricType
muom:MetricType rdf:type owl:Class ;
                rdfs:comment "The type of metric being collected, eg. Liver PDFF, patient BMI." ;
                rdfs:label "metric type" .


###  Generated by the OWL API (version 4.5.9.2019-02-01T07:24:44Z) https://github.com/owlcs/owlapi
