@prefix : <http://www.perspectum.com/ontology/scanner> .
@prefix owl: <http://www.w3.org/2002/07/owl#> .
@prefix rdf: <http://www.w3.org/1999/02/22-rdf-syntax-ns#> .
@prefix xml: <http://www.w3.org/XML/1998/namespace> .
@prefix xsd: <http://www.w3.org/2001/XMLSchema#> .
@prefix oscn: <http://www.perspectum.com/ontology/scanner#> .
@prefix qudt: <http://qudt.org/schema/qudt#> .
@prefix rdfs: <http://www.w3.org/2000/01/rdf-schema#> .
@prefix skos: <http://www.w3.org/2004/02/skos/core#> .
@prefix unit: <http://qudt.org/vocab/unit#> .
@base <http://www.perspectum.com/ontology/scanner> .

<http://www.perspectum.com/ontology/scanner> rdf:type owl:Ontology ;
                                              owl:versionIRI <http://www.perspectum.com/ontology/scanner/1.0> ;
                                              rdfs:comment """An Ontology to model MRI Scanner information.  To be used in support of an ontology of metrics collected in a clinical study of multi-organ imaging of  patients exhibiting symptoms of long Covid.

Perspectum has published a  longitudinal, observational clinical study (Dennis et al, 2020) of patients, still experiencing  symptoms 3 months post-infection, with acute SARS-CoV-2. Patients were assessed with health  questionnaires, blood investigations and quantitative magnetic resonance imaging (MRI). 

Dennis, A. et al. (2020) ‘Multi-organ impairment in low-risk individuals with long COVID’, medRxiv, p. 2020.10.14.20212555. doi: 10.1101/2020.10.14.20212555.""" ;
                                              rdfs:isDefinedBy <http://www.perspectum.com/ontology/scanner> ;
                                              rdfs:seeAlso "http://www.perspectum.com/ontology/metrics" ;
                                              owl:versionInfo """Versions

7/7/2021 1.0  First version
19/7/2021 1.1 Add ScannerFieldStrength entity
25/8/2021 1.2 Add comment annotations
14/10/2021 1.3 Add skos:altLabels; add missing comments""" .

#################################################################
#    Annotation properties
#################################################################

###  http://www.w3.org/2004/02/skos/core#altLabel
skos:altLabel rdf:type owl:AnnotationProperty .


###  http://www.w3.org/2004/02/skos/core#prefLabel
skos:prefLabel rdf:type owl:AnnotationProperty .


#################################################################
#    Object Properties
#################################################################

###  http://qudt.org/schema/qudt#unit
qudt:unit rdf:type owl:ObjectProperty ;
          rdfs:comment "unit property from QUDT ontology" ;
          rdfs:isDefinedBy <http://qudt.org/schema/qudt> ;
          rdfs:label "unit" ;
          skos:altLabel "unit"@en .


###  http://www.perspectum.com/ontology/scanner#hasFieldStrengthUnit
oscn:hasFieldStrengthUnit rdf:type owl:ObjectProperty ;
                          rdfs:subPropertyOf qudt:unit ;
                          rdfs:domain oscn:ScannerFieldStrength ;
                          rdfs:range oscn:ScannerFieldStrengthUnit ;
                          rdfs:comment "has field strength unit object property" ;
                          rdfs:isDefinedBy <http://www.perspectum.com/ontology/scanner> ;
                          rdfs:label "has field strength unit" ;
                          skos:altLabel "has unit"@en .


###  http://www.perspectum.com/ontology/scanner#hasScannerFieldStrength
oscn:hasScannerFieldStrength rdf:type owl:ObjectProperty ;
                             rdfs:domain oscn:MRIScannerModel ;
                             rdfs:range oscn:ScannerFieldStrength ;
                             rdfs:comment "object property 'has Scanner field strength' defining relationship between MRI Scanner Model and Scanner Field Strength."@en ;
                             rdfs:isDefinedBy <http://www.perspectum.com/ontology/scanner> ;
                             rdfs:label "has scanner field strength" ;
                             skos:altLabel "has field strength"@en .


###  http://www.perspectum.com/ontology/scanner#isFieldStrengthForScanner
oscn:isFieldStrengthForScanner rdf:type owl:ObjectProperty ;
                               rdfs:domain oscn:ScannerFieldStrength ;
                               rdfs:range oscn:MRIScannerModel ;
                               rdfs:comment "object property 'is field strength for scanner' defining relationship between Scanner Field Strength and MRI Scanner Model."@en ;
                               rdfs:isDefinedBy <http://www.perspectum.com/ontology/scanner> ;
                               rdfs:label "is field strength for scanner" ;
                               skos:altLabel "is field strength"@en .


###  http://www.perspectum.com/ontology/scanner#isMadeBy
oscn:isMadeBy rdf:type owl:ObjectProperty ;
              owl:inverseOf oscn:isMakerOf ;
              rdfs:comment "object property defining is made by, defining relationship between some product and a Manufacturer."@en ;
              rdfs:isDefinedBy <http://www.perspectum.com/ontology/scanner> ;
              rdfs:label "is made by" ;
              skos:altLabel "made by"@en .


###  http://www.perspectum.com/ontology/scanner#isMakerOf
oscn:isMakerOf rdf:type owl:ObjectProperty ;
               rdfs:comment "object property defining is maker of defining relationship between Manufacturer and some product."@en ;
               rdfs:isDefinedBy <http://www.perspectum.com/ontology/scanner> ;
               rdfs:label "is maker of" ;
               skos:altLabel "maker of"@en .


###  http://www.perspectum.com/ontology/scanner#isMakerOfScanner
oscn:isMakerOfScanner rdf:type owl:ObjectProperty ;
                      rdfs:subPropertyOf oscn:isMakerOf ;
                      owl:inverseOf oscn:isScannerMadeBy ;
                      rdfs:comment "object property defining is maker of scanner relationship between Scanner Manufacturer and Scanner Model."@en ;
                      rdfs:isDefinedBy <http://www.perspectum.com/ontology/scanner> ;
                      rdfs:label "is maker of scanner" ;
                      skos:altLabel "maker of"@en .


###  http://www.perspectum.com/ontology/scanner#isScannerMadeBy
oscn:isScannerMadeBy rdf:type owl:ObjectProperty ;
                     rdfs:subPropertyOf oscn:isMadeBy ;
                     rdfs:domain oscn:MRIScannerModel ;
                     rdfs:range oscn:ScannerManufacturer ;
                     rdfs:comment "object property defining is Scanner Made By relationship between Scanner Model and Scanner Manufacturer."@en ;
                     rdfs:isDefinedBy <http://www.perspectum.com/ontology/scanner> ;
                     rdfs:label "is scanner made by" ;
                     skos:altLabel "made by"@en .


#################################################################
#    Data properties
#################################################################

###  http://qudt.org/schema/qudt#value
qudt:value rdf:type owl:DatatypeProperty ;
           rdfs:comment "value data property from QUDT ontology" ;
           rdfs:isDefinedBy <http://qudt.org/schema/qudt/> ;
           rdfs:label "value" ;
           skos:altLabel "value"@en .


###  http://www.perspectum.com/ontology/scanner#FieldStrengthValue
oscn:FieldStrengthValue rdf:type owl:DatatypeProperty ;
                        rdfs:subPropertyOf qudt:value ;
                        rdfs:domain oscn:ScannerFieldStrength ;
                        rdfs:range xsd:double ;
                        rdfs:comment "Field Strength of the MRI Scanner magnet(s)" ;
                        rdfs:isDefinedBy <http://www.perspectum.com/ontology/scanner> ;
                        rdfs:label "field strength value" ;
                        skos:altLabel "field str. value"@en .


#################################################################
#    Classes
#################################################################

###  http://qudt.org/schema/qudt#Quantity
qudt:Quantity rdf:type owl:Class ;
              owl:disjointWith <http://qudt.org/schema/qudt/Unit> ,
                               oscn:MRIScannerModel ,
                               oscn:ScannerManufacturer ;
              rdfs:comment "quantity class from QUDT ontology" ;
              rdfs:isDefinedBy <http://qudt.org/schema/qudt> ;
              rdfs:label "quantity" ;
              skos:altLabel "quantity"@en .


###  http://qudt.org/schema/qudt/Unit
<http://qudt.org/schema/qudt/Unit> rdf:type owl:Class ;
                                   owl:disjointWith oscn:MRIScannerModel ,
                                                    oscn:ScannerManufacturer ;
                                   rdfs:comment "Unit of Measure from QUDT ontology" ;
                                   rdfs:isDefinedBy <http://qudt.org/schema/qudt> ;
                                   rdfs:label "Unit" ;
                                   skos:altLabel "unit"@en .


###  http://www.perspectum.com/ontology/scanner#MRIScannerModel
oscn:MRIScannerModel rdf:type owl:Class ;
                     owl:disjointWith oscn:ScannerManufacturer ;
                     rdfs:comment """An MRI ( Magnetic resonance imaging) scanner is a large tube that contains powerful magnets and can be used to examine almost any part of the body.  Magnetic resonance imaging (MRI) is a type of scan that uses strong magnetic fields and radio waves to produce detailed images of the inside of the body. The results of an MRI scan can be used to help diagnose conditions, plan treatments and assess how effective previous treatment has been.
(https://www.nhs.uk/conditions/mri-scan/)""" ;
                     rdfs:isDefinedBy <http://www.perspectum.com/ontology/scanner> ;
                     rdfs:label "MRI scanner model" ;
                     skos:altLabel "MRI scanner"@en .


###  http://www.perspectum.com/ontology/scanner#Manufacturer
oscn:Manufacturer rdf:type owl:Class .


###  http://www.perspectum.com/ontology/scanner#ScannerFieldStrength
oscn:ScannerFieldStrength rdf:type owl:Class ;
                          rdfs:subClassOf qudt:Quantity ;
                          rdfs:comment "The measure of the strength of the magnet used in an MRI Scanner." ;
                          rdfs:isDefinedBy <http://www.perspectum.com/ontology/scanner> ;
                          rdfs:label "scanner field strength" ;
                          skos:altLabel "field strength"@en .


###  http://www.perspectum.com/ontology/scanner#ScannerFieldStrengthUnit
oscn:ScannerFieldStrengthUnit rdf:type owl:Class ;
                              rdfs:subClassOf <http://qudt.org/schema/qudt/Unit> ;
                              rdfs:comment "Unit of measure of scanner field strength" ;
                              rdfs:isDefinedBy <http://qudt.org/schema/qudt> ;
                              rdfs:label "scanner field strength unit" ;
                              skos:altLabel "field str. unit"@en .


###  http://www.perspectum.com/ontology/scanner#ScannerManufacturer
oscn:ScannerManufacturer rdf:type owl:Class ;
                         rdfs:subClassOf oscn:Manufacturer ;
                         rdfs:comment "A company that manufactures and sells MR scanners for human diagnostic use." ;
                         rdfs:isDefinedBy <http://www.perspectum.com/ontology/scanner> ;
                         rdfs:label "scanner manufacturer" ;
                         skos:altLabel "manufacturer"@en .


###  Generated by the OWL API (version 4.5.9.2019-02-01T07:24:44Z) https://github.com/owlcs/owlapi
